Finish proof of endpoint to payload semantics preservation

projection/proofs/endpoint_to_payloadProofScript.sml
@@ -16,6 +16,267 @@ val compile_queue_lift_ineq = Q.store_thm("compile_queue_lift_ineq",
   >> fs[compile_queue_def]
   >> simp[EVERY_MAP]);
 
+val list_trans_def = Define `
+    (list_trans conf p [] q = (p = q))
+ /\ (list_trans conf p (alpha::l) q = ?p'. trans conf p alpha p' /\ list_trans conf p' l q)`
+
+val list_trans_par_l = Q.store_thm("list_trans_par_l",
+  `∀conf p alpha q r. list_trans conf p alpha q ==> list_trans conf (NPar p r) alpha (NPar q r)`,
+  Induct_on `alpha`
+  >- simp[list_trans_def]
+  >> rpt strip_tac
+  >> fs[list_trans_def] >> metis_tac[payloadSemanticsTheory.trans_par_l])
+
+val list_trans_par_r = Q.store_thm("list_trans_par_r",
+  `∀conf p alpha q r. list_trans conf p alpha q ==> list_trans conf (NPar r p) alpha (NPar r q)`,
+  Induct_on `alpha`
+  >- simp[list_trans_def]
+  >> rpt strip_tac
+  >> fs[list_trans_def] >> metis_tac[payloadSemanticsTheory.trans_par_r])
+
+val compile_message_preservation_send = Q.store_thm("compile_message_preservation_send",
+  `∀conf d p1 p2 e s.
+    conf.payload_size > 0
+    ∧ p1 ≠ p2
+    ==> list_trans conf
+        (NEndpoint p1 s
+         (Send p2 (INR d) e))
+        (MAP (λm. LSend p1 m p2) (compile_message conf d))
+        (NEndpoint p1 s e)
+  `,
+  recInduct compile_message_ind
+  >> rpt strip_tac
+  >> PURE_ONCE_REWRITE_TAC [compile_message_def]
+  >> simp[]
+  >> IF_CASES_TAC
+  >- (simp[list_trans_def] >> match_mp_tac trans_send_last_payload >> simp[])
+  >- (fs[list_trans_def,NOT_LESS_EQUAL]
+      >> drule(trans_send_intermediate_payload|>REWRITE_RULE[GREATER_DEF])
+      >> disch_then drule
+      >> disch_then(qspecl_then [`s`,`e`] assume_tac)
+      >> asm_exists_tac
+      >> simp[]))
+
+val compile_network_preservation_send = Q.store_thm("compile_network_preservation_send",
+  `∀p1 p2 q1 d q2 conf.
+    conf.payload_size > 0
+    ∧ trans p1 (LSend q1 d q2) p2
+    ==> list_trans conf (compile_network conf p1)
+                        (LTau::MAP (λm. LSend q1 m q2) (compile_message conf d))
+                        (compile_network conf p2)
+  `,
+  rpt strip_tac
+  >> qpat_x_assum `conf.payload_size > 0` mp_tac
+  >> qmatch_asmsub_abbrev_tac `trans _ alpha _`
+  >> pop_assum (mp_tac o PURE_ONCE_REWRITE_RULE [markerTheory.Abbrev_def])
+  >> MAP_EVERY (W(curry Q.SPEC_TAC)) [`q1`,`d`,`q2`,`conf`]
+  >> pop_assum mp_tac
+  >> MAP_EVERY (W(curry Q.SPEC_TAC)) [`p2`,`alpha`,`p1`]
+  >> ho_match_mp_tac trans_ind
+  >> rpt strip_tac
+  >> fs[] >> rveq
+  >- ((* trans_send *)
+      simp[compile_network_def,compile_endpoint_def,list_trans_def]
+      >> qexists_tac `NEndpoint p1 (s with queue := compile_queue conf s.queue)
+                      (Send p2 (INR d) (compile_endpoint e))`
+      >> conj_tac
+      >- (match_mp_tac trans_send_var >> simp[])
+      >- (match_mp_tac compile_message_preservation_send >> simp[]))
+  >- ((* trans_par_l *)
+      first_x_assum drule >> simp[compile_network_def] >> MATCH_ACCEPT_TAC list_trans_par_l)
+  >- ((* trans_par_r *)
+      first_x_assum drule >> simp[compile_network_def] >> MATCH_ACCEPT_TAC list_trans_par_r));
+
+val compile_message_preservation_enqueue = Q.store_thm("compile_message_preservation_enqueue",
+  `∀conf d q p1 p2 e s.
+    conf.payload_size > 0
+    ∧ p1 ≠ p2
+    ==> list_trans conf
+  (NEndpoint p2 (s with queue := q) e)
+  (MAP (λm. LReceive p1 m p2) (compile_message conf d))
+  (NEndpoint p2
+     (s with queue := q ⧺ MAP (λd. (p1,d)) (compile_message conf d)) e)
+  `,
+  recInduct compile_message_ind
+  >> rpt strip_tac
+  >> PURE_ONCE_REWRITE_TAC [compile_message_def]
+  >> simp[]
+  >> IF_CASES_TAC
+  >- (simp[list_trans_def] >> drule payloadSemanticsTheory.trans_enqueue >> simp[SNOC_APPEND]
+      >> disch_then(qspecl_then [`conf`,`s with queue := q`] mp_tac)
+      >> simp[])
+  >- (fs[list_trans_def,NOT_LESS_EQUAL]
+      >> drule payloadPropsTheory.trans_enqueue'
+      >> disch_then (qspecl_then [`conf`,`s`,`2w::TAKE conf.payload_size d`,`e`,`q`] assume_tac)
+      >> asm_exists_tac >> simp[]
+      >> first_x_assum drule
+      >> disch_then (qspec_then `q ++ [(p1,2w::TAKE conf.payload_size d)]` assume_tac)
+      >> full_simp_tac std_ss [GSYM APPEND_ASSOC,APPEND,SNOC_APPEND]));
+
+val compile_network_preservation_receive = Q.store_thm("compile_network_preservation_receive",
+  `∀p1 p2 q1 d q2 conf.
+    conf.payload_size > 0
+    ∧ trans p1 (LReceive q1 d q2) p2
+    ==> list_trans conf (compile_network conf p1)
+                        (MAP (λm. LReceive q1 m q2) (compile_message conf d))
+                        (compile_network conf p2)
+  `,
+  rpt strip_tac
+  >> qpat_x_assum `conf.payload_size > 0` mp_tac
+  >> qmatch_asmsub_abbrev_tac `trans _ alpha _`
+  >> pop_assum (mp_tac o PURE_ONCE_REWRITE_RULE [markerTheory.Abbrev_def])
+  >> MAP_EVERY (W(curry Q.SPEC_TAC)) [`q1`,`d`,`q2`,`conf`]
+  >> pop_assum mp_tac
+  >> MAP_EVERY (W(curry Q.SPEC_TAC)) [`p2`,`alpha`,`p1`]
+  >> ho_match_mp_tac trans_ind
+  >> rpt strip_tac
+  >> fs[] >> rveq
+  >- ((* trans_enqueue *)
+      simp[compile_network_def,compile_endpoint_def,SNOC_APPEND,compile_queue_append,
+           compile_queue_def,compile_message_preservation_enqueue])
+  >- ((* trans_par_l *)
+      first_x_assum drule >> simp[compile_network_def] >> MATCH_ACCEPT_TAC list_trans_par_l)
+  >- ((* trans_par_r *)
+      first_x_assum drule >> simp[compile_network_def] >> MATCH_ACCEPT_TAC list_trans_par_r));
+
+val compile_network_preservation_com_l = Q.store_thm("compile_network_preservation_com_l",
+  `∀conf d p1 p2 r1 r2 q1 q2.
+    conf.payload_size > 0
+    ∧ q1 ≠ q2
+    ∧ list_trans conf p1
+                        (MAP (λm. LSend q1 m q2) d)
+                        p2
+    ∧ list_trans conf r1
+                        (MAP (λm. LReceive q1 m q2) d)
+                        r2
+    ==> (reduction conf)^* (NPar p1 r1) (NPar p2 r2)
+  `,
+  Induct_on `d` >> rpt strip_tac
+  >> fs[list_trans_def]
+  >> match_mp_tac (RTC_RULES |> SPEC_ALL |> CONJUNCT2)
+  >> imp_res_tac payloadSemanticsTheory.trans_com_l
+  >> simp [payloadSemanticsTheory.reduction_def]
+  >> asm_exists_tac
+  >> simp[] >> metis_tac[])
+
+val compile_network_preservation_com_r = Q.store_thm("compile_network_preservation_com_r",
+  `∀conf d p1 p2 r1 r2 q1 q2.
+    conf.payload_size > 0
+    ∧ q1 ≠ q2
+    ∧ list_trans conf p1
+                        (MAP (λm. LReceive q1 m q2) d)
+                        p2
+    ∧ list_trans conf r1
+                        (MAP (λm. LSend q1 m q2) d)
+                        r2
+    ==> (reduction conf)^* (NPar p1 r1) (NPar p2 r2)
+  `,
+  Induct_on `d` >> rpt strip_tac
+  >> fs[list_trans_def]
+  >> match_mp_tac (RTC_RULES |> SPEC_ALL |> CONJUNCT2)
+  >> imp_res_tac payloadSemanticsTheory.trans_com_r
+  >> simp [payloadSemanticsTheory.reduction_def]
+  >> asm_exists_tac
+  >> simp[] >> metis_tac[])
+
+val compile_network_preservation_int_choice = Q.store_thm("compile_network_preservation_int_choice",
+  `∀p1 p2 q1 b q2 conf.
+    trans p1 (LIntChoice q1 b q2) p2
+    ==> trans conf (compile_network conf p1) (LIntChoice q1 b q2) (compile_network conf p2)
+  `,
+  rpt strip_tac
+  >> qmatch_asmsub_abbrev_tac `trans _ alpha _`
+  >> pop_assum (mp_tac o PURE_ONCE_REWRITE_RULE [markerTheory.Abbrev_def])
+  >> MAP_EVERY (W(curry Q.SPEC_TAC)) [`q1`,`b`,`q2`,`conf`]
+  >> pop_assum mp_tac
+  >> MAP_EVERY (W(curry Q.SPEC_TAC)) [`p2`,`alpha`,`p1`]
+  >> ho_match_mp_tac trans_ind
+  >> rpt strip_tac
+  >> fs[] >> rveq
+  >- ((* trans_int_choice *)
+      simp[compile_network_def,compile_endpoint_def]
+      >> match_mp_tac payloadSemanticsTheory.trans_int_choice
+      >> rw[])
+  >- ((* trans_par_l *)
+      simp[compile_network_def]
+      >> metis_tac[payloadSemanticsTheory.trans_par_l])
+  >- ((* trans_par_r *)
+      simp[compile_network_def]
+      >> metis_tac[payloadSemanticsTheory.trans_par_r]));
+
+val compile_network_preservation_ext_choice = Q.store_thm("compile_network_preservation_ext_choice",
+  `∀p1 p2 q1 b q2 conf.
+    conf.payload_size > 0 /\ trans p1 (LExtChoice q1 b q2) p2
+    ==> trans conf (compile_network conf p1) (LExtChoice q1 b q2) (compile_network conf p2)
+  `,
+  rpt strip_tac
+  >> qpat_x_assum `_.payload_size > _` mp_tac
+  >> qmatch_asmsub_abbrev_tac `trans _ alpha _`
+  >> pop_assum (mp_tac o PURE_ONCE_REWRITE_RULE [markerTheory.Abbrev_def])
+  >> MAP_EVERY (W(curry Q.SPEC_TAC)) [`q1`,`b`,`q2`,`conf`]
+  >> pop_assum mp_tac
+  >> MAP_EVERY (W(curry Q.SPEC_TAC)) [`p2`,`alpha`,`p1`]
+  >> ho_match_mp_tac trans_ind
+  >> rpt strip_tac
+  >> fs[] >> rveq
+  >- ((* trans_enqueue_choice_l *)
+     simp[compile_network_def,compile_endpoint_def,SNOC_APPEND,compile_queue_append,
+          compile_queue_def]
+     >> PURE_ONCE_REWRITE_TAC [compile_message_def]
+     >> fs[] >> fs[GSYM SNOC_APPEND]
+     >> match_mp_tac trans_enqueue_choice_l' >> rw[])
+  >- ((* trans_enqueue_choice_r *)
+     simp[compile_network_def,compile_endpoint_def,SNOC_APPEND,compile_queue_append,
+          compile_queue_def]
+     >> PURE_ONCE_REWRITE_TAC [compile_message_def]
+     >> fs[] >> fs[GSYM SNOC_APPEND]
+     >> match_mp_tac trans_enqueue_choice_r' >> rw[])
+  >- ((* trans_par_l *)
+      simp[compile_network_def]
+      >> metis_tac[payloadSemanticsTheory.trans_par_l])
+  >- ((* trans_par_r *)
+      simp[compile_network_def]
+      >> metis_tac[payloadSemanticsTheory.trans_par_r]));
+
+val MAP_TL_compile_message = Q.store_thm("MAP_TL_compile_message",
+  `!conf d. conf.payload_size > 0 ==> FLAT(MAP TL (compile_message conf d)) = d`,
+  recInduct compile_message_ind
+  >> rpt strip_tac
+  >> PURE_ONCE_REWRITE_TAC [compile_message_def]
+  >> rw[])
+  
+val compile_message_preservation_dequeue = Q.store_thm("compile_message_preservation_dequeue",
+  `!conf d ds p1 p2 q1 q2 e s v.
+   p1 ≠ p2 /\ conf.payload_size > 0 /\ EVERY (λ(p,_). p ≠ p1) q1
+   ==>                                                                                       
+   (reduction conf)^*
+    (NEndpoint p2
+               (s with queue := q1 ⧺ MAP (λd. (p1,d)) (compile_message conf d) ⧺ q2)
+               (Receive p1 v ds e))
+    (NEndpoint p2
+               <|bindings := s.bindings |+ (v,FLAT(ds) ++ d);
+                 queue := q1 ⧺ q2|>
+               e)`,
+  recInduct compile_message_ind
+  >> rpt strip_tac
+  >> PURE_ONCE_REWRITE_TAC[compile_message_def]
+  >> simp[]
+  >> IF_CASES_TAC
+  >- (match_mp_tac RTC_SINGLE
+      >> simp[payloadSemanticsTheory.reduction_def]
+      >> drule trans_dequeue_last_payload'
+      >> disch_then drule >> simp[SNOC_APPEND])
+  >- (match_mp_tac (RTC_RULES |> SPEC_ALL |> CONJUNCT2)
+      >> fs[] >> first_x_assum drule >> disch_then drule
+      >> disch_then(qspecl_then [`ds ++ [TAKE conf.payload_size d]`,
+                    `q2`,`e`,`s`,`v`] assume_tac)
+      >> PURE_ONCE_REWRITE_TAC [CONJ_SYM]
+      >> fs[] >> FULL_SIMP_TAC std_ss [GSYM APPEND_ASSOC,TAKE_DROP]
+      >> asm_exists_tac >> simp[]
+      >> simp[payloadSemanticsTheory.reduction_def]
+      >> drule trans_dequeue_intermediate_payload'
+      >> disch_then drule >> FULL_SIMP_TAC std_ss [GSYM APPEND_ASSOC,APPEND,SNOC_APPEND]));
+
 val compile_network_preservation_trans = Q.store_thm("compile_network_preservation_trans",
   `∀p1 p2 conf.
     conf.payload_size > 0
@@ -31,12 +292,48 @@ val compile_network_preservation_trans = Q.store_thm("compile_network_preservati
   >> pop_assum mp_tac
   >> MAP_EVERY (W(curry Q.SPEC_TAC)) [`p2`,`alpha`,`p1`]
   >> ho_match_mp_tac endpointSemanticsTheory.trans_strongind
-  >> rpt strip_tac >> fs[]
-  >- cheat
-  >- cheat
-  >- cheat
-  >- cheat
-  >- cheat
+  >> rpt strip_tac >> fs[] >> rveq
+  >- ((* trans_com_l *)
+      MAP_EVERY imp_res_tac [compile_network_preservation_send,
+                             compile_network_preservation_receive]
+      >> fs[list_trans_def]
+      >> match_mp_tac (RTC_RULES |> SPEC_ALL |> CONJUNCT2)
+      >> PURE_ONCE_REWRITE_TAC [CONJ_SYM]
+      >> imp_res_tac compile_network_preservation_com_l
+      >> simp[compile_network_def] >> asm_exists_tac
+      >> simp[payloadSemanticsTheory.reduction_def]
+      >> match_mp_tac payloadSemanticsTheory.trans_par_l
+      >> simp[])
+  >- ((* trans_com_r *)
+      MAP_EVERY imp_res_tac [compile_network_preservation_send,
+                             compile_network_preservation_receive]
+      >> fs[list_trans_def]
+      >> match_mp_tac (RTC_RULES |> SPEC_ALL |> CONJUNCT2)
+      >> PURE_ONCE_REWRITE_TAC [CONJ_SYM]
+      >> imp_res_tac compile_network_preservation_com_r
+      >> simp[compile_network_def] >> asm_exists_tac
+      >> simp[payloadSemanticsTheory.reduction_def]
+      >> match_mp_tac payloadSemanticsTheory.trans_par_r
+      >> simp[])
+  >- ((* trans_com_choice_l *)
+      MAP_EVERY imp_res_tac [compile_network_preservation_ext_choice,
+                             compile_network_preservation_int_choice]
+      >> match_mp_tac RTC_SINGLE >> simp[payloadSemanticsTheory.reduction_def]
+      >> simp[compile_network_def]
+      >> metis_tac[payloadSemanticsTheory.trans_com_choice_l])
+  >- ((* trans_com_choice_r *)
+      MAP_EVERY imp_res_tac [compile_network_preservation_ext_choice,
+                             compile_network_preservation_int_choice]
+      >> match_mp_tac RTC_SINGLE >> simp[payloadSemanticsTheory.reduction_def]
+      >> simp[compile_network_def]
+      >> metis_tac[payloadSemanticsTheory.trans_com_choice_r])
+  >- ((* trans_dequeue *)
+       simp[compile_network_def,compile_endpoint_def,compile_queue_def,compile_queue_append]
+       >> drule compile_message_preservation_dequeue
+       >> drule compile_queue_lift_ineq >> disch_then(qspec_then `conf` assume_tac)
+       >> disch_then drule >> disch_then drule
+       >> disch_then(qspecl_then [`d`,`[]`] mp_tac)
+       >> simp[])
   >- ((* trans_ext_choice_l *)
       fs[compile_network_def,compile_queue_def,compile_endpoint_def,compile_queue_append]
       >> PURE_ONCE_REWRITE_TAC[compile_message_def]
